almost done (without challenge 2); some errors on byte/int conversions, can not write

src/Challenge 3/find_k_smallest.dfy
@@ -5,11 +5,223 @@
  * have the Kth smallest numbers.  
  */
 
+/* 
+ * Building command:
+ * 
+ * dafny build find_k_smallest.dfy IoNative.cs --unicode-char:false
+ */
+
+/* 
+ * Running commands (examples):
+ *
+ * ./find_k_smallest.exe 5 SourceFile DestFile
+ * (or)
+ * dotnet find_k_smallest.dll 5 SourceFile DestFile
+ */
+
 include "Io.dfy"
+
+function IsInteger(chars: array<char>): bool
+  reads chars
+{
+  // Check each character in the array
+  forall i :: 0 <= i < chars.Length ==> '0' <= chars[i] <= '9'
+}
+
+method CharArrayToInt(arr: array<char>) returns (n: int)
+  requires IsInteger(arr)
+{
+  var k := 0;
+  var mult := 1;
+  var i := arr.Length - 1;
+
+  while (i >= 0)
+  {
+    k := k + (arr[i] as int  - '0' as int) * mult;
+    mult := mult * 10;
+    i := i - 1;
+  }
+
+  return k;
+}
+
+method ByteArrayToIntArray(a:array<byte>) returns (b: array<int32>)
+  //ensures forall i :: 0 <= i < b.Length ==> 0 <= b[i] < 256
+  ensures b.Length == a.Length
+{
+  b := new int32[a.Length];
+
+  for i := 0 to a.Length
+  {
+    b[i] := a[i] as int32 - 48;
+  }
+}
+
+method IntArrayToByteArray(a:array<int32>) returns (b: array<byte>)
+  requires forall i :: 0 <= i < a.Length ==> 0 <= a[i] < 256
+  ensures b.Length == a.Length
+{
+  b := new byte[a.Length];
+
+  for i := 0 to a.Length
+  {
+    b[i] := a[i] as byte;
+  }
+}
 
 method {:main} Main(ghost env:HostEnvironment?)
   requires env != null && env.Valid() && env.ok.ok()
+  modifies env.ok, env.files
 {
-  print "TODO!\n";  
-}
+  // - First step -
+  // Read the command line
 
+  // Check the number of arguments
+  var numArgs := HostConstants.NumCommandLineArgs(env);
+
+  // If number of arguments is different than 4, print error message
+  if numArgs != 4
+  {
+    print "Error: Wrong number of arguments!\nUsage: number sourceFile destFile";
+    return;
+  }
+
+  // Verify argument 1 - number
+  // (first verification will only verify if it is a number)
+  // (later it will verify if the number is between the correct range)
+
+  var argNumber := HostConstants.GetCommandLineArg(1, env);
+
+  if !IsInteger(argNumber)
+  {
+    print "Error: Wrong argument type! Argument 1 must be of type int!\nUsage: number sourceFile destFile";
+    return;
+  }
+
+  // Convert the number variable (char array) into 
+  var number: int := CharArrayToInt(argNumber);
+
+  // Verify argument 2 - source file
+
+  var sourceFile := HostConstants.GetCommandLineArg(2, env);
+
+  // Verify if source file exists
+
+  var sourceFileExists := FileStream.FileExists(sourceFile, env);
+
+  if !sourceFileExists
+  {
+    print "Error: Source file does not exist!";
+    return;
+  }
+
+  // Verify argument 3 - destination file
+
+  var destFile := HostConstants.GetCommandLineArg(3, env);
+
+  // Verify if destination file already exists
+
+  var destFileExists := FileStream.FileExists(destFile, env);
+
+  if destFileExists
+  {
+    print "Error: Destination file already exists!";
+    return;
+  }
+
+  // - Second step -
+  // Open, read from and close the source file
+
+  // Open source file
+
+  var ok: bool;
+  var sourceFileStream: FileStream?;
+
+  ok, sourceFileStream := FileStream.Open(sourceFile, env);
+
+  if !ok
+  {
+    print "Error: Could not open source file!";
+    return;
+  }
+
+  // Get the length of the source file
+  
+  var len: int32;
+
+  ok, len := FileStream.FileLength(sourceFile, env);
+
+  if !ok {
+    print "Error: Could not get the length of the source file!";
+    return;
+  }
+
+  // Create a buffer to read the file content
+
+  var buffer := new byte[len];
+
+  // Read the content of the source file into the buffer
+
+  ok := sourceFileStream.Read(0, buffer, 0, len);
+
+  if !ok {
+    print "Error: Could not read from source file!";
+    return;
+  }
+
+  // Convert the byte array to an int array
+
+  var numbers := ByteArrayToIntArray(buffer);
+
+  // Close the source file
+
+  ok := sourceFileStream.Close();
+
+  if !ok {
+    print "Error: Could not close source file!";
+    return;
+  }
+
+  // - Third step -
+  // Apply method from Challenge 2
+
+  //------------------------------
+
+  // - Forth and final step -
+  // Create, write to and close destination file
+
+  // Create/open destination file
+
+  var destFileStream: FileStream?;
+
+  ok, destFileStream := FileStream.Open(destFile, env);
+
+  if !ok
+  {
+    print "Error: Could not create destination file!";
+    return;
+  }
+
+  // Convert the int array to a byte array
+
+  var numbersByteArray := IntArrayToByteArray(numbers);
+
+  // Write the byte array to the destination file
+
+  ok := destFileStream.Write(0, numbersByteArray, 0, len);
+
+  if !ok
+  {
+    print "Error: Could not write to destination file!";
+    return;
+  }
+
+  // Close the destination file
+
+  ok := destFileStream.Close();
+
+  if !ok {
+    print "Error: Could not close destination file!";
+    return;
+  }
+}
